Move sort client to right file.

theories/examples/sort.v
@@ -30,11 +30,6 @@ Definition sort_service : val :=
     "xs" <- lmerge "cmp" !"ys" !"zs";;
     send "c" #().
 
-Definition sort_client : val := λ: "cmp" "xs",
-  let: "c" := start_chan sort_service in
-  send "c" "cmp";; send "c" "xs";;
-  recv "c".
-
 Section sort.
   Context `{!heapG Σ, !proto_chanG Σ} (N : namespace).
 
@@ -120,23 +115,5 @@ Section sort.
       + by apply (Sorted_list_merge _).
       + rewrite (merge_Permutation R). by f_equiv.
     - by iApply "HΨ".
-  Qed.
-
-  Lemma sort_client_spec {A} (I : A → val → iProp Σ) R
-       `{!RelDecision R, !Total R} cmp l (vs : list val) (xs : list A) :
-    cmp_spec I R cmp -∗
-    {{{ l ↦ llist vs ∗ [∗ list] x;v ∈ xs;vs, I x v }}}
-      sort_client cmp #l
-    {{{ ys ws, RET #(); ⌜Sorted R ys⌝ ∗ ⌜ys ≡ₚ xs⌝ ∗
-               l ↦ llist ws ∗ [∗ list] y;w ∈ ys;ws, I y w }}}.
-  Proof.
-    iIntros "#Hcmp !>" (Φ) "Hl HΦ". wp_lam.
-    wp_apply (start_chan_proto_spec N sort_protocol); iIntros (c) "Hc".
-    { rewrite -(right_id END%proto _ (iProto_dual _)).
-      wp_apply (sort_service_spec with "Hc"); auto. }
-    wp_send with "[$Hcmp]".
-    wp_send with "[$Hl]".
-    wp_recv (ys ws) as "(Hsorted & Hperm & Hl & HI)".
-    wp_pures. iApply "HΦ"; iFrame.
   Qed.
 End sort.
