theories/examples/sort_client.v
@@ -1,19 +1,42 @@
 From stdpp Require Import sorting.
-From osiris.channel Require Import proto_channel.
+From osiris.channel Require Import proto_channel proofmode.
 From iris.heap_lang Require Import proofmode notation.
 From osiris.utils Require Import list compare.
 From osiris.examples Require Import sort.
 
+Definition sort_client : val := λ: "cmp" "xs",
+  let: "c" := start_chan sort_service in
+  send "c" "cmp";; send "c" "xs";;
+  recv "c".
+
 Section sort_client.
   Context `{!heapG Σ, !proto_chanG Σ} (N : namespace).
 
-  Lemma sort_client_le_spec l (xs : list Z) :
+  Lemma sort_client_spec {A} (I : A → val → iProp Σ) R
+       `{!RelDecision R, !Total R} cmp l (vs : list val) (xs : list A) :
+    cmp_spec I R cmp -∗
+    {{{ l ↦ llist vs ∗ [∗ list] x;v ∈ xs;vs, I x v }}}
+      sort_client cmp #l
+    {{{ ys ws, RET #(); ⌜Sorted R ys⌝ ∗ ⌜ys ≡ₚ xs⌝ ∗
+               l ↦ llist ws ∗ [∗ list] y;w ∈ ys;ws, I y w }}}.
+  Proof.
+    iIntros "#Hcmp !>" (Φ) "Hl HΦ". wp_lam.
+    wp_apply (start_chan_proto_spec N sort_protocol); iIntros (c) "Hc".
+    { rewrite -(right_id END%proto _ (iProto_dual _)).
+      wp_apply (sort_service_spec with "Hc"); auto. }
+    wp_send with "[$Hcmp]".
+    wp_send with "[$Hl]".
+    wp_recv (ys ws) as "(Hsorted & Hperm & Hl & HI)".
+    wp_pures. iApply "HΦ"; iFrame.
+  Qed.
+
+  Lemma sort_client_Zle_spec l (xs : list Z) :
     {{{ l ↦ llist (LitV ∘ LitInt <$> xs) }}}
       sort_client cmpZ #l
     {{{ ys, RET #(); ⌜Sorted (≤) ys⌝ ∗ ⌜ ys ≡ₚ xs⌝ ∗ l ↦ llist (LitV ∘ LitInt <$> ys) }}}.
   Proof.
     iIntros (Φ) "Hl HΦ".
-    iApply (sort_client_spec N IZ (≤) _ _ (LitV ∘ LitInt <$> xs) xs with "[] [Hl] [HΦ]").
+    iApply (sort_client_spec IZ (≤) _ _ (LitV ∘ LitInt <$> xs) xs with "[] [Hl] [HΦ]").
     { iApply cmpZ_spec. }
     { iFrame "Hl". iInduction xs as [|x xs] "IH"; csimpl; by iFrame "#". }
     iIntros "!>" (ys ws) "(?&?&?&HI)".
